more

operations/Unique_Fixpoint_Data.thy
@@ -6,6 +6,55 @@ declare supp_id_bound[simp] supp_inv_bound[simp] infinite_UNIV[simp]
 
 definition "IImsupp' Inj Vr \<rho> = SSupp Inj \<rho> \<union> IImsupp Inj Vr \<rho>"
 
+typedecl Gbd_type
+consts Gbd :: "Gbd_type rel"
+
+setup \<open>Sign.mandatory_path "G"\<close>
+axiomatization where
+  infinite_regular_card_order: "infinite_regular_card_order Gbd"
+setup \<open>Sign.parent_path\<close>
+
+class covar =
+  assumes large: "cardSuc Gbd \<le>o |UNIV::'a set|"
+    and regular: "regularCard |UNIV::'a set|"
+
+class var =
+  assumes large: "|Field Gbd| \<le>o |UNIV::'a set|"
+    and regular: "regularCard |UNIV::'a set|"
+
+instantiation Gbd_type :: var begin
+instance apply standard
+  apply simp
+  by (meson G.infinite_regular_card_order card_of_unique
+      card_order_on_Card_order infinite_regular_card_order_def
+      regularCard_ordIso)
+end
+
+subclass (in covar) var
+  apply standard
+  apply (meson cardSuc_ordLess_ordLeq card_of_Card_order
+      card_of_Field_ordIso G.infinite_regular_card_order
+      infinite_regular_card_order.Card_order local.large
+      ordIso_ordLeq_trans ordLeq_iff_ordLess_or_ordIso)
+  by (rule local.regular)
+
+subclass (in var) infinite
+  apply standard
+  using card_of_ordLeq_finite cinfinite_def
+    G.infinite_regular_card_order
+    infinite_regular_card_order.cinfinite local.large
+  by auto
+
+lemma large': "Gbd \<le>o |UNIV::'a::var set|"
+  using Card_order_iff_ordLeq_card_of var_class.large
+    G.infinite_regular_card_order infinite_regular_card_order.Card_order ordLeq_transitive
+  by blast
+
+lemma (in var) UN_bound: "|A| <o |UNIV::'a set| \<Longrightarrow> (\<And>x. x \<in> A \<Longrightarrow> |f x| <o |UNIV::'a set| )
+  \<Longrightarrow> |\<Union>(f ` A)| <o |UNIV::'a set|"
+  using card_of_Card_order card_of_UNION_ordLess_infinite_Field local.regular regularCard_stable
+  by (metis Field_card_of infinite_UNIV)
+
 lemma IImsupp_bound[simp]:
   "|SSupp Inj (\<rho> :: 'a::var \<Rightarrow> _)| <o |UNIV :: 'a set| \<Longrightarrow> (\<And>x. |Vr (\<rho> x)| <o |UNIV :: 'a set| ) \<Longrightarrow>
   |IImsupp' Inj (Vr :: _ \<Rightarrow> 'a set) \<rho>| <o |UNIV :: 'a set|"
@@ -21,21 +70,9 @@ consts GSupp1 :: "('a1 :: var, 'a2 :: var, 'x1, 'x2) G \<Rightarrow> 'x1 set"
 consts GSupp2 :: "('a1 :: var, 'a2 :: var, 'x1, 'x2) G \<Rightarrow> 'x2 set"
 consts Gwit :: "('a1, 'a2, 'x1, 'x2) G"
 
-(*
-declare [[goals_limit = 20]]
-pbmv_monad "('a1::var, 'a2::var, 'x1, 'x2) G"
-  Sbs: Gsub
-  RVrs: GVrs1 GVrs2
-  Maps: Gmap
-  Supps: GSupp1 GSupp2
-  bd: natLeq
-  oops
-*)
-
 setup \<open>Sign.mandatory_path "G"\<close>
 
 axiomatization where
-  infinite_regular_card_order: "infinite_regular_card_order natLeq" and
   Sb_Inj: "Gsub id id = id" and
   Sb_comp: "\<And>g1 g2 f1 f2.
        |supp (f1 :: 'a1::var \<Rightarrow> 'a1)| <o |UNIV :: 'a1 set| \<Longrightarrow>
@@ -43,8 +80,8 @@ axiomatization where
        |supp (g1 :: 'a1::var \<Rightarrow> 'a1)| <o |UNIV :: 'a1 set| \<Longrightarrow>
        |supp (g2 :: 'a2::var \<Rightarrow> 'a2)| <o |UNIV :: 'a2 set| \<Longrightarrow>
        Gsub g1 g2 \<circ> Gsub f1 f2 = Gsub (g1 \<circ> f1) (g2 \<circ> f2)" and
-  Vrs1_bd: "(\<And>x. |GVrs1 x| <o natLeq)" and
-  Vrs2_bd: "(\<And>x. |GVrs2 x| <o natLeq)" and
+  Vrs1_bd: "(\<And>x. |GVrs1 x| <o Gbd)" and
+  Vrs2_bd: "(\<And>x. |GVrs2 x| <o Gbd)" and
   Vrs1_Sb: "(\<And>f1 f2 x.
        |supp (f1 :: 'a1::var \<Rightarrow> 'a1)| <o |UNIV :: 'a1 set| \<Longrightarrow>
        |supp (f2 :: 'a2::var \<Rightarrow> 'a2)| <o |UNIV :: 'a2 set| \<Longrightarrow> GVrs1 (Gsub f1 f2 x) = f1 ` GVrs1 x)" and
@@ -63,8 +100,8 @@ axiomatization where
   Map_comp: "\<And>f1 f2 g1 g2. Gmap g1 g2 \<circ> Gmap f1 f2 = Gmap (g1 \<circ> f1) (g2 \<circ> f2)" and
   Supp1_Map: "(\<And>f1 f2 x. GSupp1 (Gmap f1 f2 x) = f1 ` GSupp1 x)" and
   Supp2_Map: "(\<And>f1 f2 x. GSupp2 (Gmap f1 f2 x) = f2 ` GSupp2 x)" and
-  Supp1_bd: "(\<And>x. |GSupp1 x| <o natLeq)" and
-  Supp2_bd:  "(\<And>x. |GSupp2 x| <o natLeq)" and
+  Supp1_bd: "(\<And>x. |GSupp1 x| <o Gbd)" and
+  Supp2_bd:  "(\<And>x. |GSupp2 x| <o Gbd)" and
   Map_cong: "\<And>f1 f2 g1 g2 x.
         (\<And>a. a \<in> GSupp1 x \<Longrightarrow> f1 a = g1 a) \<Longrightarrow>
         (\<And>a. a \<in> GSupp2 x \<Longrightarrow> f2 a = g2 a) \<Longrightarrow>
@@ -92,19 +129,20 @@ lemmas Vrs_Map = G.Vrs_Map1 G.Vrs_Map2
 setup \<open>Sign.parent_path\<close>
 
 (* In this case the flat version, Gren, happens to be the same as Gsub. *)
-abbreviation Gren :: 
+definition Gren :: 
   "('a1 :: var \<Rightarrow> 'a1) \<Rightarrow> ('a2 :: var \<Rightarrow> 'a2) \<Rightarrow> ('a1, 'a2, 'c1, 'c2) G \<Rightarrow> ('a1, 'a2, 'c1, 'c2) G" where 
-  "Gren \<rho>1 \<rho>2 u \<equiv> Gsub \<rho>1 \<rho>2 u"
+  "Gren \<rho>1 \<rho>2 u = Gsub \<rho>1 \<rho>2 u"
 
 definition "GMAP = (\<lambda>\<rho>1 \<rho>2 f1 f2 x. Gren \<rho>1 \<rho>2 (Gmap f1 f2 x))"
 
+declare [[typedef_overloaded]]
 mrbnf "('a1::var, 'a2::var, 'x1, 'x2) G"
   map: GMAP
   sets: free: GVrs1 bound: GVrs2 live: GSupp1 live: GSupp2
-  bd: natLeq
+  bd: Gbd
   wits: Gwit
+  var_class: var
   sorry
-
 print_theorems
 
 consts \<eta> :: "'a1 :: var \<Rightarrow> ('a1, 'a2 :: var, 'x1, 'x2) G"
@@ -112,14 +150,14 @@ consts \<eta>' :: "'a1 :: var \<Rightarrow> ('a1, 'a2 :: var, 'x1, 'x2) G"
 
 axiomatization where
   eta_inversion: "\<And>\<delta>1 \<delta>2 f1 f2 u a. |supp \<delta>1| <o |UNIV::'a1 set| \<Longrightarrow> |supp \<delta>2| <o |UNIV::'a2 set| \<Longrightarrow>
-   Gren \<delta>1 \<delta>2 (Gmap f1 f2 u) = (\<eta> a :: ('a1::var, 'a2 :: var, 'x1, 'x2) G) \<Longrightarrow> \<exists>y. u = \<eta> y"
+   Gsub \<delta>1 \<delta>2 (Gmap f1 f2 u) = (\<eta> a :: ('a1::var, 'a2 :: var, 'x1, 'x2) G) \<Longrightarrow> \<exists>y. u = \<eta> y"
   and eta_natural: "\<And>\<delta>1 \<delta>2 f1 f2 a. |supp \<delta>1| <o |UNIV::'a1 set| \<Longrightarrow> |supp \<delta>2| <o |UNIV::'a2 set| \<Longrightarrow>
-   Gren \<delta>1 \<delta>2 (Gmap f1 f2 (\<eta> a :: ('a1::var, 'a2 :: var, 'x1, 'x2) G)) = \<eta> (\<delta>1 a)"
+   Gsub \<delta>1 \<delta>2 (Gmap f1 f2 (\<eta> a :: ('a1::var, 'a2 :: var, 'x1, 'x2) G)) = \<eta> (\<delta>1 a)"
   and eta_mem: "\<And>a. a \<in> GVrs1 (\<eta> a :: ('a1::var, 'a2 :: var, 'x1, 'x2) G)"
   and eta'_inversion: "\<And>\<delta>1 \<delta>2 f1 f2 u a. |supp \<delta>1| <o |UNIV::'a1 set| \<Longrightarrow> |supp \<delta>2| <o |UNIV::'a2 set| \<Longrightarrow>
-   Gren \<delta>1 \<delta>2 (Gmap f1 f2 u) = \<eta>' a \<Longrightarrow> \<exists>y. u = \<eta>' y"
+   Gsub \<delta>1 \<delta>2 (Gmap f1 f2 u) = \<eta>' a \<Longrightarrow> \<exists>y. u = \<eta>' y"
   and eta'_natural: "\<And>\<delta>1 \<delta>2 f1 f2 a. |supp \<delta>1| <o |UNIV::'a1 set| \<Longrightarrow> |supp \<delta>2| <o |UNIV::'a2 set| \<Longrightarrow>
-   Gren \<delta>1 \<delta>2 (Gmap f1 f2 (\<eta>' a :: ('a1::var, 'a2 :: var, 'x1, 'x2) G)) = \<eta>' (\<delta>1 a)"
+   Gsub \<delta>1 \<delta>2 (Gmap f1 f2 (\<eta>' a :: ('a1::var, 'a2 :: var, 'x1, 'x2) G)) = \<eta>' (\<delta>1 a)"
   and eta'_mem: "\<And>a. a \<in> GVrs1 (\<eta>' a :: ('a1::var, 'a2 :: var, 'x1, 'x2) G)"
   and eta_inj: "\<And>a a'. \<eta> a = \<eta> a' \<Longrightarrow> a = a'"
   and eta'_inj: "\<And>a a'. \<eta>' a = \<eta>' a' \<Longrightarrow> a = a'"
@@ -148,10 +186,13 @@ proof safe
        apply (simp_all add: G.Vrs_Sb)
       apply (auto simp: swap_def)
       done
-    with b have False
-      apply simp
-      by (smt (verit) G.Vrs_bd(1) UNIV_cinfinite UNIV_eq_I
-          cinfinite_imp_infinite eta_mem finite_iff_ordLess_natLeq)
+    with b have "|UNIV - {a}| \<le>o |GVrs1 (\<eta> a :: ('a1 ::var, 'a2 :: var, 'x1, 'x2) G)|"
+      by (intro card_of_mono1) auto
+    then have "|UNIV::'a1 set| \<le>o |GVrs1 (\<eta> a :: ('a1 ::var, 'a2 :: var, 'x1, 'x2) G)|"
+      by (meson infinite_UNIV infinite_card_of_diff_singl ordIso_ordLeq_trans ordIso_symmetric)
+    then have False
+      using G.Vrs_bd(1) large' not_ordLeq_ordLess
+        ordLeq_ordLess_trans by blast
   }
   then show "b = a"
     by blast
@@ -163,7 +204,7 @@ next
   then have "GVrs2 (\<eta> a :: ('a1 ::var, 'a2 :: var, 'x1, 'x2) G) = UNIV"
     by blast
   then show "b \<in> {}"
-    by (metis G.Vrs_bd(2) finite_iff_ordLess_natLeq infinite_UNIV)
+    by (metis G.Vrs_bd(2) large' exists_fresh exists_univ_eq ordLess_ordLeq_trans)
 qed (rule eta_mem)
 
 lemma GVrs_eta'[simp]:
@@ -181,10 +222,13 @@ proof safe
        apply (simp_all add: G.Vrs_Sb)
       apply (auto simp: swap_def)
       done
-    with b have False
-      apply simp
-      by (smt (verit) G.Vrs_bd(1) UNIV_cinfinite UNIV_eq_I
-          cinfinite_imp_infinite eta'_mem finite_iff_ordLess_natLeq)
+    with b have "|UNIV - {a}| \<le>o |GVrs1 (\<eta>' a :: ('a1 ::var, 'a2 :: var, 'x1, 'x2) G)|"
+      by (intro card_of_mono1) auto
+    then have "|UNIV::'a1 set| \<le>o |GVrs1 (\<eta>' a :: ('a1 ::var, 'a2 :: var, 'x1, 'x2) G)|"
+      by (meson infinite_UNIV infinite_card_of_diff_singl ordIso_ordLeq_trans ordIso_symmetric)
+    then have False
+      using G.Vrs_bd(1) large' not_ordLeq_ordLess
+        ordLeq_ordLess_trans by blast
   }
   then show "b = a"
     by blast
@@ -196,7 +240,7 @@ next
   then have "GVrs2 (\<eta>' a :: ('a1 ::var, 'a2 :: var, 'x1, 'x2) G) = UNIV"
     by blast
   then show "b \<in> {}"
-    by (metis G.Vrs_bd(2) finite_iff_ordLess_natLeq infinite_UNIV)
+    by (metis G.Vrs_bd(2) large' exists_fresh exists_univ_eq ordLess_ordLeq_trans)
 qed (rule eta'_mem)
 
 lemma GSupp_eta[simp]:
@@ -204,22 +248,28 @@ lemma GSupp_eta[simp]:
   "GSupp2 (\<eta> a :: ('a1 ::var, 'a2 :: var, 'x1, 'x2) G) = {}"
 proof safe
   fix b :: 'x1 assume "b \<in> GSupp1 (\<eta> a :: ('a1 ::var, 'a2 :: var, 'x1, 'x2) G)"
-  then have "c \<in> GSupp1 (\<eta> a :: ('a1 ::var, 'a2 :: var, nat, 'x2) G)" for c :: nat
-    by (subst eta_natural[of id id "\<lambda>x. if x = b then c else 0" id a, symmetric, simplified])
+  then have "c \<in> GSupp1 (\<eta> a :: ('a1 ::var, 'a2 :: var, Gbd_type, 'x2) G)" for c :: Gbd_type
+    by (subst eta_natural[of id id "\<lambda>x. if x = b then c else (undefined :: Gbd_type)" id a, symmetric, simplified])
       (auto simp: G.Supp_Sb  G.Supp_Map image_iff intro!: bexI[of _ b])
-  then have "GSupp1 (\<eta> a :: ('a1 ::var, 'a2 :: var, nat, 'x2) G) = UNIV"
+  then have "GSupp1 (\<eta> a :: ('a1 ::var, 'a2 :: var, Gbd_type, 'x2) G) = UNIV"
     by blast
-  then show "b \<in> {}"
-    by (metis G.Supp_bd(1) finite_iff_ordLess_natLeq infinite_UNIV)
+  moreover have "|UNIV :: Gbd_type set| =o Gbd"
+    using card_of_unique G.infinite_regular_card_order
+      infinite_regular_card_order.card_order ordIso_symmetric by blast
+  ultimately show "b \<in> {}"
+    by (metis G.Supp_bd(1) not_ordLess_ordIso)
 next
   fix b :: 'x2 assume "b \<in> GSupp2 (\<eta> a :: ('a1 ::var, 'a2 :: var, 'x1, 'x2) G)"
-  then have "c \<in> GSupp2 (\<eta> a :: ('a1 ::var, 'a2 :: var, 'x1, nat) G)" for c :: nat
-    by (subst eta_natural[of id id id "\<lambda>x. if x = b then c else 0" a, symmetric, simplified])
+  then have "c \<in> GSupp2 (\<eta> a :: ('a1 ::var, 'a2 :: var, 'x1, Gbd_type) G)" for c :: Gbd_type
+    by (subst eta_natural[of id id id "\<lambda>x. if x = b then c else (undefined :: Gbd_type)" a, symmetric, simplified])
       (auto simp: G.Supp_Sb  G.Supp_Map image_iff intro!: bexI[of _ b])
-  then have "GSupp2 (\<eta> a :: ('a1 ::var, 'a2 :: var, 'x1, nat) G) = UNIV"
+  then have "GSupp2 (\<eta> a :: ('a1 ::var, 'a2 :: var, 'x1, Gbd_type) G) = UNIV"
     by blast
-  then show "b \<in> {}"
-    by (metis G.Supp_bd(2) finite_iff_ordLess_natLeq infinite_UNIV)
+  moreover have "|UNIV :: Gbd_type set| =o Gbd"
+    using card_of_unique G.infinite_regular_card_order
+      infinite_regular_card_order.card_order ordIso_symmetric by blast
+  ultimately show "b \<in> {}"
+    by (metis G.Supp_bd(2) not_ordLess_ordIso)
 qed
 
 lemma GSupp_eta'[simp]:
@@ -227,55 +277,66 @@ lemma GSupp_eta'[simp]:
   "GSupp2 (\<eta>' a :: ('a1 ::var, 'a2 :: var, 'x1, 'x2) G) = {}"
 proof safe
   fix b :: 'x1 assume "b \<in> GSupp1 (\<eta>' a :: ('a1 ::var, 'a2 :: var, 'x1, 'x2) G)"
-  then have "c \<in> GSupp1 (\<eta>' a :: ('a1 ::var, 'a2 :: var, nat, 'x2) G)" for c :: nat
-    by (subst eta'_natural[of id id "\<lambda>x. if x = b then c else 0" id a, symmetric, simplified])
+  then have "c \<in> GSupp1 (\<eta>' a :: ('a1 ::var, 'a2 :: var, Gbd_type, 'x2) G)" for c :: Gbd_type
+    by (subst eta'_natural[of id id "\<lambda>x. if x = b then c else (undefined :: Gbd_type)" id a, symmetric, simplified])
       (auto simp: G.Supp_Sb  G.Supp_Map image_iff intro!: bexI[of _ b])
-  then have "GSupp1 (\<eta>' a :: ('a1 ::var, 'a2 :: var, nat, 'x2) G) = UNIV"
+  then have "GSupp1 (\<eta>' a :: ('a1 ::var, 'a2 :: var, Gbd_type, 'x2) G) = UNIV"
     by blast
-  then show "b \<in> {}"
-    by (metis G.Supp_bd(1) finite_iff_ordLess_natLeq infinite_UNIV)
+  moreover have "|UNIV :: Gbd_type set| =o Gbd"
+    using card_of_unique G.infinite_regular_card_order
+      infinite_regular_card_order.card_order ordIso_symmetric by blast
+  ultimately show "b \<in> {}"
+    by (metis G.Supp_bd(1) not_ordLess_ordIso)
 next
   fix b :: 'x2 assume "b \<in> GSupp2 (\<eta>' a :: ('a1 ::var, 'a2 :: var, 'x1, 'x2) G)"
-  then have "c \<in> GSupp2 (\<eta>' a :: ('a1 ::var, 'a2 :: var, 'x1, nat) G)" for c :: nat
-    by (subst eta'_natural[of id id id "\<lambda>x. if x = b then c else 0" a, symmetric, simplified])
-      (auto simp: G.Supp_Sb  G.Supp_Map image_iff intro!: bexI[of _ b])
-  then have "GSupp2 (\<eta>' a :: ('a1 ::var, 'a2 :: var, 'x1, nat) G) = UNIV"
+  then have "c \<in> GSupp2 (\<eta>' a :: ('a1 ::var, 'a2 :: var, 'x1, Gbd_type) G)" for c :: Gbd_type
+    by (subst eta'_natural[of id id id "\<lambda>x. if x = b then c else (undefined :: Gbd_type)" a, symmetric, simplified])
+      (auto simp: G.Supp_Sb G.Supp_Map image_iff intro!: bexI[of _ b])
+  then have "GSupp2 (\<eta>' a :: ('a1 ::var, 'a2 :: var, 'x1, Gbd_type) G) = UNIV"
     by blast
-  then show "b \<in> {}"
-    by (metis G.Supp_bd(2) finite_iff_ordLess_natLeq infinite_UNIV)
+  moreover have "|UNIV :: Gbd_type set| =o Gbd"
+    using card_of_unique G.infinite_regular_card_order
+      infinite_regular_card_order.card_order ordIso_symmetric by blast
+  ultimately show "b \<in> {}"
+    by (metis G.Supp_bd(2) not_ordLess_ordIso)
 qed
 
 declare [[typedef_overloaded]]
 binder_datatype (EVrs: 'a) E = Ector "('a, x::'a, t::'a E, 'a E) G" binds x in t
   for permute: Eperm
-
 declare E.inject[simp del]
+
+(*for technical reasons we now work with var_E_pre but the classes are the same*)
+sublocale var_E_pre < var
+  by (rule var_axioms)
+sublocale var < var_E_pre
+  by standard
 
 lemma
   Eperm_comp:
-  "\<And>\<sigma> \<tau>. bij (\<sigma> :: 'a :: var \<Rightarrow> 'a) \<Longrightarrow> |supp \<sigma>| <o |UNIV :: 'a set| \<Longrightarrow>
-   bij (\<tau> :: 'a :: var \<Rightarrow> 'a) \<Longrightarrow> |supp \<tau>| <o |UNIV :: 'a set| \<Longrightarrow>
+  "\<And>\<sigma> \<tau>. bij (\<sigma> :: 'a :: var_E_pre \<Rightarrow> 'a) \<Longrightarrow> |supp \<sigma>| <o |UNIV :: 'a set| \<Longrightarrow>
+   bij (\<tau> :: 'a :: var_E_pre \<Rightarrow> 'a) \<Longrightarrow> |supp \<tau>| <o |UNIV :: 'a set| \<Longrightarrow>
    Eperm \<sigma> o Eperm \<tau> = Eperm (\<sigma> o \<tau>)"
   and EVrs_Eperm:
-  "\<And>\<sigma> u. bij (\<sigma> :: 'a :: var \<Rightarrow> 'a) \<Longrightarrow> |supp \<sigma>| <o |UNIV :: 'a set| \<Longrightarrow> 
+  "\<And>\<sigma> u. bij (\<sigma> :: 'a :: var_E_pre \<Rightarrow> 'a) \<Longrightarrow> |supp \<sigma>| <o |UNIV :: 'a set| \<Longrightarrow> 
    EVrs (Eperm \<sigma> u) \<subseteq> \<sigma> ` EVrs u"
   and Eperm_cong_id:
-  "\<And>\<sigma> e. bij (\<sigma> :: 'a :: var \<Rightarrow> 'a) \<Longrightarrow> |supp \<sigma>| <o |UNIV :: 'a set| \<Longrightarrow>
+  "\<And>\<sigma> e. bij (\<sigma> :: 'a :: var_E_pre \<Rightarrow> 'a) \<Longrightarrow> |supp \<sigma>| <o |UNIV :: 'a set| \<Longrightarrow>
    (\<And>a. a \<in> EVrs e \<Longrightarrow> \<sigma> a = a) \<Longrightarrow> Eperm \<sigma> e = e"
   and Eperm_Ector:
-  "\<And>\<sigma> u. bij (\<sigma> :: 'a :: var \<Rightarrow> 'a) \<Longrightarrow> |supp \<sigma>| <o |UNIV :: 'a set| \<Longrightarrow>
-    Eperm \<sigma> (Ector u) = Ector (Gsub \<sigma> \<sigma> (Gmap (Eperm \<sigma>) (Eperm \<sigma>) u))"
+  "\<And>\<sigma> u. bij (\<sigma> :: 'a :: var_E_pre \<Rightarrow> 'a) \<Longrightarrow> |supp \<sigma>| <o |UNIV :: 'a set| \<Longrightarrow>
+    Eperm \<sigma> (Ector u) = Ector (Gren \<sigma> \<sigma> (Gmap (Eperm \<sigma>) (Eperm \<sigma>) u))"
   and Ector_inject: "\<And>x y. (Ector x = Ector y) =
-   (\<exists>\<sigma> :: 'a :: var \<Rightarrow> 'a. bij \<sigma> \<and> |supp \<sigma>| <o |UNIV :: 'a set| \<and>
-     id_on (\<Union> (EVrs ` GSupp1 x) - GVrs2 x) \<sigma> \<and> Gsub id \<sigma> (Gmap (Eperm \<sigma>) id x) = y)"
-  and Ector_fresh_surj: "\<And>A e. |A::'a set| <o |UNIV :: 'a::var set| \<Longrightarrow> 
+   (\<exists>\<sigma> :: 'a :: var_E_pre \<Rightarrow> 'a. bij \<sigma> \<and> |supp \<sigma>| <o |UNIV :: 'a set| \<and>
+     id_on (\<Union> (EVrs ` GSupp1 x) - GVrs2 x) \<sigma> \<and> Gren id \<sigma> (Gmap (Eperm \<sigma>) id x) = y)"
+  and Ector_fresh_surj: "\<And>A e. |A::'a set| <o |UNIV :: 'a::var_E_pre set| \<Longrightarrow> 
     \<exists>u. GVrs2 u \<inter> A = {} \<and> e = Ector u"
   and EVrs_Ector:
-  "\<And>u. EVrs (Ector u::('a::var) E) =
+  "\<And>u. EVrs (Ector u::('a::var_E_pre) E) =
      GVrs1 u \<union> ((\<Union>e \<in> GSupp1 u. EVrs e) - GVrs2 u) \<union> (\<Union>e \<in> GSupp2 u. EVrs e)"
   and EVrs_bd:
-  "\<And>x. |EVrs (x :: 'a :: var E)| <o natLeq"
-          apply (auto simp: E.inject E.permute_id0 E.permute_comp E.FVars_permute GMAP_def E.FVars_bd
+  "\<And>x. |EVrs (x :: 'a :: var_E_pre E)| <o Gbd"
+          apply (auto simp: E.inject E.permute_id0 E.permute_comp E.FVars_permute GMAP_def Gren_def E.FVars_bd
              intro: E.permute_cong_id)
   subgoal for A e
     apply (binder_induction e avoiding: A rule: E.strong_induct)
@@ -284,20 +345,6 @@ lemma
      apply assumption
     apply (rule refl)
     done
-  done
-
-lemma Eperm_id: "Eperm id = id"
-  apply (rule ext)
-  apply (rule trans[OF Eperm_cong_id id_apply[symmetric]])
-    apply simp_all
-  done
-
-lemma Eperm_cong: "bij (\<sigma> :: 'a :: var \<Rightarrow> 'a) \<Longrightarrow> |supp \<sigma>| <o |UNIV :: 'a set| \<Longrightarrow>
-         bij (\<tau> :: 'a :: var \<Rightarrow> 'a) \<Longrightarrow> |supp \<tau>| <o |UNIV :: 'a set| \<Longrightarrow>
-   (\<And>a. a \<in> EVrs e \<Longrightarrow> \<sigma> a = \<tau> a) \<Longrightarrow> Eperm \<sigma> e = Eperm \<tau> e"
-  apply (rule trans[OF _ Eperm_cong_id, of _ "\<sigma> o inv \<tau>"])
-     apply (auto simp: Eperm_comp[THEN fun_cong, simplified] supp_comp_bound
-       dest: EVrs_Eperm[THEN set_mp, rotated -1] simp flip: o_assoc)
   done
 
 inductive subshape where
@@ -322,7 +369,7 @@ lemma subshape_induct: "(\<And>e. (\<And>e'. subshape e' e \<Longrightarrow> P e
   by (metis wfp_induct)
 
 lemma E_coinduct:
-  fixes P and g :: "'k \<Rightarrow> 'a::var E" and h e
+  fixes P and g :: "'k \<Rightarrow> 'a::var_E_pre E" and h e
   assumes "(\<And>k. P k \<Longrightarrow> g k = h k \<or>
     (\<exists>u. g k = Ector (GMAP id id g g u) \<and> h k = Ector (GMAP id id h h u) \<and>
     (\<forall>k \<in> GSupp1 u. P k) \<and> (\<forall>k \<in> GSupp2 u. P k)))"
@@ -353,18 +400,18 @@ lemma E_coinduct:
   done
 
 context
-  fixes \<delta> :: "'a \<Rightarrow> 'a :: var" and \<rho> \<rho>' :: "'a ::var \<Rightarrow> 'a E"
+  fixes \<delta> :: "'a \<Rightarrow> 'a :: var_E_pre" and \<rho> \<rho>' :: "'a ::var_E_pre \<Rightarrow> 'a E"
   assumes small_support:
-    "|supp (\<delta> :: 'a \<Rightarrow> 'a :: var)| <o |UNIV::'a set|"
-    "|SSupp (Ector o \<eta>) (\<rho>::'a::var \<Rightarrow> 'a E)| <o |UNIV::'a set|"
-    "|SSupp (Ector o \<eta>') (\<rho>'::'a::var \<Rightarrow> 'a E)| <o |UNIV::'a set|"
+    "|supp (\<delta> :: 'a \<Rightarrow> 'a :: var_E_pre)| <o |UNIV::'a set|"
+    "|SSupp (Ector o \<eta>) (\<rho>::'a::var_E_pre \<Rightarrow> 'a E)| <o |UNIV::'a set|"
+    "|SSupp (Ector o \<eta>') (\<rho>'::'a::var_E_pre \<Rightarrow> 'a E)| <o |UNIV::'a set|"
 begin
 
 lemma permute_\<rho>:
   "bij f \<Longrightarrow> |supp f| <o |UNIV :: 'a set| \<Longrightarrow> imsupp f \<inter> IImsupp' (Ector \<circ> \<eta>) EVrs \<rho> = {} \<Longrightarrow> Eperm f (\<rho> a) = \<rho> (f a)"
   apply (cases "f a = a")
    apply (cases "\<rho> a = Ector (\<eta> a)")
-    apply (simp add: GMAP_def eta_natural)
+    apply (simp add: GMAP_def Gren_def eta_natural)
    apply simp
    apply (rule E.permute_cong_id; simp?)
   subgoal for a'
@@ -373,7 +420,7 @@ lemma permute_\<rho>:
     apply (auto simp: IImsupp'_def IImsupp_def SSupp_def)
     done
   apply (cases "\<rho> a = Ector (\<eta> a)")
-   apply (simp add: GMAP_def eta_natural)
+   apply (simp add: GMAP_def Gren_def eta_natural)
    apply (auto simp: IImsupp'_def IImsupp_def SSupp_def imsupp_def supp_def)
   done
 
@@ -381,7 +428,7 @@ lemma permute_\<rho>':
   "bij f \<Longrightarrow> |supp f| <o |UNIV :: 'a set| \<Longrightarrow> imsupp f \<inter> IImsupp' (Ector \<circ> \<eta>') EVrs \<rho>' = {} \<Longrightarrow> Eperm f (\<rho>' a) = \<rho>' (f a)"
   apply (cases "f a = a")
    apply (cases "\<rho>' a = Ector (\<eta>' a)")
-    apply (simp add: GMAP_def eta'_natural)
+    apply (simp add: GMAP_def Gren_def eta'_natural)
    apply simp
    apply (rule E.permute_cong_id; simp?)
   subgoal for a'
@@ -390,7 +437,7 @@ lemma permute_\<rho>':
     apply (auto simp: IImsupp'_def IImsupp_def SSupp_def)
     done
   apply (cases "\<rho>' a = Ector (\<eta>' a)")
-   apply (simp add: GMAP_def eta'_natural)
+   apply (simp add: GMAP_def Gren_def eta'_natural)
    apply (auto simp: IImsupp'_def IImsupp_def SSupp_def imsupp_def supp_def)
   done
 
@@ -402,7 +449,7 @@ interpretation Esub: QREC_fixed_E "imsupp \<delta> \<union> IImsupp' (Ector o \<
     apply (auto intro!: Un_bound simp: E.FVars_bd_UNIVs imsupp_supp_bound small_support) []
    apply (auto simp: map_E_pre_def set2_E_pre_def set3_E_pre_def set4_E_pre_def
      permute_\<rho> permute_\<rho>'
-     Abs_E_pre_inverse GMAP_def eta_natural eta'_natural small_support imsupp_commute[of _ \<delta>]
+     Abs_E_pre_inverse GMAP_def Gren_def eta_natural eta'_natural small_support imsupp_commute[of _ \<delta>]
      G.Map_Sb[THEN fun_cong, simplified]
      G.Sb_comp[THEN fun_cong, simplified]
      G.Map_comp[THEN fun_cong, simplified] G.Supp_Map G.Supp_Sb G.Vrs_Map G.Vrs_Sb
@@ -435,19 +482,19 @@ lemma
     apply (subst (2) Ector_def)
     apply (subst Esub.REC_ctor)
       apply (auto simp: map_E_pre_def set2_E_pre_def Abs_E_pre_inverse noclash_E_def
-        eta_distinct GMAP_def eta_natural eta_inject)
+        eta_distinct GMAP_def Gren_def eta_natural eta_inject)
     done
   subgoal
     apply (subst (2) Ector_def)
     apply (subst Esub.REC_ctor)
       apply (auto simp: map_E_pre_def set2_E_pre_def Abs_E_pre_inverse noclash_E_def
-        eta_distinct' GMAP_def eta'_natural eta'_inject)
+        eta_distinct' GMAP_def Gren_def eta'_natural eta'_inject)
     done
   subgoal
     apply (subst (2) Ector_def)
     apply (subst Esub.REC_ctor)
       apply (auto simp: map_E_pre_def set1_E_pre_def set2_E_pre_def set3_E_pre_def set4_E_pre_def
-        GMAP_def eta_distinct Abs_E_pre_inverse noclash_E_def small_support comp_def[of snd]
+        GMAP_def Gren_def eta_distinct Abs_E_pre_inverse noclash_E_def small_support comp_def[of snd]
         G.Map_Sb[THEN fun_cong, simplified]
         G.Sb_comp[THEN fun_cong, simplified]
         G.Map_comp[THEN fun_cong, simplified]
@@ -468,8 +515,22 @@ lemma Eperm_Esub: "bij f \<Longrightarrow> |supp f| <o |UNIV :: 'a set| \<Longri
 
 end
 
+lemma Eperm_id: "Eperm id = id"
+  apply (rule ext)
+  apply (rule trans[OF Eperm_cong_id id_apply[symmetric]])
+    apply simp_all
+  done
+
+lemma Eperm_cong: "bij (\<sigma> :: 'a :: var_E_pre \<Rightarrow> 'a) \<Longrightarrow> |supp \<sigma>| <o |UNIV :: 'a set| \<Longrightarrow>
+         bij (\<tau> :: 'a :: var_E_pre \<Rightarrow> 'a) \<Longrightarrow> |supp \<tau>| <o |UNIV :: 'a set| \<Longrightarrow>
+   (\<And>a. a \<in> EVrs e \<Longrightarrow> \<sigma> a = \<tau> a) \<Longrightarrow> Eperm \<sigma> e = Eperm \<tau> e"
+  apply (rule trans[OF _ Eperm_cong_id, of _ "\<sigma> o inv \<tau>"])
+     apply (auto simp: Eperm_comp[THEN fun_cong, simplified] supp_comp_bound
+       dest: EVrs_Eperm[THEN set_mp, rotated -1] simp flip: o_assoc)
+  done
+
 lemma Ector_eta_inj: "Ector u = Ector (\<eta> a) \<longleftrightarrow> u = \<eta> a"
-  by (metis Ector_inject eta_natural supp_id_bound)
+  by (metis Ector_inject eta_natural supp_id_bound Gren_def)
 
 lemma Ector_eta'_inj: "Ector u = Ector (\<eta>' a) \<longleftrightarrow> u = \<eta>' a"
   unfolding Ector_inject
@@ -478,10 +539,10 @@ lemma Ector_eta'_inj: "Ector u = Ector (\<eta>' a) \<longleftrightarrow> u = \<e
     apply (drule arg_cong[where f = "Gsub id (inv \<sigma>) o Gmap (Eperm (inv \<sigma>)) id"])
     apply (auto simp: eta'_natural G.Map_comp[THEN fun_cong, simplified]
         G.Map_Sb[THEN fun_cong, simplified] G.Sb_comp[THEN fun_cong, simplified]
-        G.Map_id G.Sb_Inj Eperm_comp Eperm_id)
+        G.Map_id G.Sb_Inj Eperm_comp Eperm_id Gren_def)
     done
   subgoal
-    apply (auto simp: eta'_natural)
+    apply (auto simp: eta'_natural Gren_def)
     done
   done
 
@@ -491,11 +552,14 @@ lemma Ector_eta_inj': "Ector (\<eta> a) = Ector x \<longleftrightarrow> x = \<et
 lemma Ector_eta'_inj': "Ector (\<eta>' a) = Ector x \<longleftrightarrow> x = \<eta>' a"
   using Ector_eta'_inj by metis
 
-lemma EVrs_bound[simp]: "|EVrs (x :: 'a :: var E)| <o |UNIV :: 'a set|"
-  by (meson EVrs_bd var_class.large' ordLess_ordLeq_trans)
+lemma EVrs_bound[simp]: "|EVrs (x :: 'a :: var_E_pre E)| <o |UNIV :: 'a set|"
+  by (rule ordLess_ordLeq_trans[OF EVrs_bd large'])
+
+lemma GVrs2_bound[simp]: "|GVrs2 (u::('a :: var_E_pre, 'a, 'a E, 'a E) G)| <o |UNIV :: 'a set|"
+  by (rule ordLess_ordLeq_trans[OF G.Vrs_bd(2) large'])
 
 lemma Ector_fresh_inject:
-  assumes "GVrs2 x \<inter> A = {}" "GVrs2 y \<inter> A = {}" "|A :: 'a::var set| <o |UNIV :: 'a set|"
+  assumes "GVrs2 x \<inter> A = {}" "GVrs2 y \<inter> A = {}" "|A :: 'a::var_E_pre set| <o |UNIV :: 'a set|"
   shows "(Ector x = Ector y) = (\<exists>\<sigma>. bij \<sigma> \<and> |supp \<sigma>| <o |UNIV :: 'a set| \<and> imsupp \<sigma> \<inter> A = {}
     \<and> id_on (\<Union> (EVrs ` GSupp1 x) - GVrs2 x) \<sigma> \<and> Gren id \<sigma> (Gmap (Eperm \<sigma>) id x) = y)"
   unfolding Ector_inject
@@ -505,7 +569,7 @@ lemma Ector_fresh_inject:
     apply (drule meta_mp; simp add: UN_bound card_of_minus_bound ordLess_ordLeq_trans[OF G.Supp_bd(1) large'] ordLess_ordLeq_trans[OF G.Vrs_bd(2) large'] assms)+
     apply (elim exE conjE)
     subgoal for \<tau>
-      apply (auto simp: G.Vrs_Map intro!: exI[of _ \<tau>] trans[OF G.Sb_cong arg_cong[where f="Gren _ _", OF G.Map_cong]] Eperm_cong)
+      apply (auto simp: G.Vrs_Map Gren_def intro!: exI[of _ \<tau>] trans[OF G.Sb_cong arg_cong[where f="Gsub _ _", OF G.Map_cong]] Eperm_cong)
       using G.Vrs_Map(2) G.Vrs_Sb(2) assms(2) imageI supp_id_bound apply blast
       apply (smt (verit, ccfv_threshold) Diff_iff G.Vrs_Map(2) G.Vrs_Sb(2) UN_I assms(2) disjoint_iff_not_equal id_on_eq imageI supp_id_bound)
       done
@@ -514,9 +578,9 @@ lemma Ector_fresh_inject:
   done
 
 lemma Esub_inversion0:
-  "|supp (\<delta> :: 'a \<Rightarrow> 'a :: var)| <o |UNIV::'a set| \<Longrightarrow>
-   |SSupp (Ector o \<eta>) (\<rho>::'a::var \<Rightarrow> 'a E)| <o |UNIV::'a set| \<Longrightarrow>
-   |SSupp (Ector o \<eta>') (\<rho>'::'a::var \<Rightarrow> 'a E)| <o |UNIV::'a set| \<Longrightarrow>
+  "|supp (\<delta> :: 'a \<Rightarrow> 'a :: var_E_pre)| <o |UNIV::'a set| \<Longrightarrow>
+   |SSupp (Ector o \<eta>) (\<rho>::'a::var_E_pre \<Rightarrow> 'a E)| <o |UNIV::'a set| \<Longrightarrow>
+   |SSupp (Ector o \<eta>') (\<rho>'::'a::var_E_pre \<Rightarrow> 'a E)| <o |UNIV::'a set| \<Longrightarrow>
    GVrs2 u \<inter> (imsupp \<delta> \<union> IImsupp' (Ector o \<eta>) EVrs \<rho> \<union> IImsupp' (Ector o \<eta>') EVrs \<rho>' \<union> EVrs e \<union> EVrs (Ector u)) = {} \<Longrightarrow>
    \<forall>a. e \<noteq> Ector (\<eta> a) \<Longrightarrow> \<forall>a. e \<noteq> Ector (\<eta>' a) \<Longrightarrow>
    \<forall>a. u \<noteq> \<eta> a \<Longrightarrow> \<forall>a. u \<noteq> \<eta>' a \<Longrightarrow>
@@ -530,34 +594,29 @@ lemma Esub_inversion0:
   apply (drule sym)
   subgoal for u'
     apply (subst (asm) Ector_fresh_inject[where A = "imsupp \<delta> \<union> IImsupp' (Ector o \<eta>) EVrs \<rho> \<union> IImsupp' (Ector o \<eta>') EVrs \<rho>' \<union> (\<Union> (EVrs ` GSupp1 u') - GVrs2 u')"])
-       apply (simp_all add: Int_Un_distrib G.Vrs_Sb G.Vrs_Map) [2]
-     apply (auto intro!: Un_bound UN_bound card_of_minus_bound simp: imsupp_supp_bound ordLess_ordLeq_trans[OF G.Supp_bd(1) large']) []
+       apply (simp_all add: Int_Un_distrib G.Vrs_Sb G.Vrs_Map EVrs_Ector) [2]
+      apply (auto intro!: Un_bound UN_bound card_of_minus_bound simp: imsupp_supp_bound ordLess_ordLeq_trans[OF G.Supp_bd(1) large']) []
     apply (erule exE conjE)+
     subgoal for \<sigma>
-      apply (rule exI[where x = "GMAP id \<sigma> (Eperm \<sigma>) id u'"])
+      apply (rule exI[where x = "Gren id \<sigma> (Gmap (Eperm \<sigma>) id u')"])
       apply (rule conjI)
        apply (erule trans[OF sym])
-       apply (auto 0 0 simp add: Int_Un_distrib GMAP_def G.Map_Sb[THEN fun_cong, simplified] G.Sb_comp[THEN fun_cong, simplified] G.Map_comp[THEN fun_cong, simplified] Eperm_Esub Ector_inject
-          G.Vrs_Sb G.Vrs_Map intro!: trans[OF G.Sb_cong arg_cong[where f = "Gren _ _", OF G.Map_cong]] exI[of _ \<sigma>])
+       apply (auto 0 0 simp add: Int_Un_distrib G.Map_Sb[THEN fun_cong, simplified] G.Sb_comp[THEN fun_cong, simplified] G.Map_comp[THEN fun_cong, simplified] Eperm_Esub Ector_inject
+          G.Vrs_Sb G.Vrs_Map Gren_def intro!: trans[OF G.Sb_cong arg_cong[where f = "Gsub _ _", OF G.Map_cong]] exI[of _ \<sigma>])
       apply (meson disjoint_iff_not_equal id_on_def not_in_imsupp_same)
       done
     done
   done
 
 lemma Esub_inversion:
-  "|supp (\<delta> :: 'a \<Rightarrow> 'a :: var)| <o |UNIV::'a set| \<Longrightarrow>
-   |SSupp (Ector o \<eta>) (\<rho>::'a::var \<Rightarrow> 'a E)| <o |UNIV::'a set| \<Longrightarrow>
-   |SSupp (Ector o \<eta>') (\<rho>'::'a::var \<Rightarrow> 'a E)| <o |UNIV::'a set| \<Longrightarrow>
+  "|supp (\<delta> :: 'a \<Rightarrow> 'a :: var_E_pre)| <o |UNIV::'a set| \<Longrightarrow>
+   |SSupp (Ector o \<eta>) (\<rho>::'a::var_E_pre \<Rightarrow> 'a E)| <o |UNIV::'a set| \<Longrightarrow>
+   |SSupp (Ector o \<eta>') (\<rho>'::'a::var_E_pre \<Rightarrow> 'a E)| <o |UNIV::'a set| \<Longrightarrow>
    GVrs2 u \<inter> (imsupp \<delta> \<union> IImsupp' (Ector o \<eta>) EVrs \<rho> \<union> IImsupp' (Ector o \<eta>') EVrs \<rho>' \<union> EVrs e) = {} \<Longrightarrow>
    \<forall>a. e \<noteq> Ector (\<eta> a) \<Longrightarrow> \<forall>a. e \<noteq> Ector (\<eta>' a) \<Longrightarrow>
    \<forall>a. u \<noteq> \<eta> a \<Longrightarrow> \<forall>a. u \<noteq> \<eta>' a \<Longrightarrow>
    Ector u = Esub \<delta> \<rho> \<rho>' e \<Longrightarrow> \<exists>u'. u = Gsub \<delta> id (Gmap (Esub \<delta> \<rho> \<rho>') (Esub \<delta> \<rho> \<rho>') u') \<and> GVrs2 u' = GVrs2 u \<and> e = Ector u'"
   by (rule Esub_inversion0) (auto dest!: set_mp[OF EVrs_Esub, rotated -1])
-
-declare GMAP_def[simp]
-
-lemma GVrs2_bound[simp]: "|GVrs2 (u::('a :: var, 'a, 'a E, 'a E) G)| <o |UNIV :: 'a set|"
-  by (meson G.Vrs_bd var_class.large' ordLess_ordLeq_trans)
 
 inductive Efreee where 
   GVrs1: "a \<in> GVrs1 u \<Longrightarrow> \<forall>a. u \<noteq> \<eta> a \<Longrightarrow> \<forall>a'. u \<noteq> \<eta>' a' \<Longrightarrow> Efreee a (Ector u)"
@@ -575,7 +634,7 @@ binder_inductive (no_auto_equiv) Efreee
     subgoal for _ u
       apply (rule exI[of _ "\<sigma> a"])
       apply (rule exI[of _ "Gsub \<sigma> \<sigma> (Gmap (Eperm \<sigma>) (Eperm \<sigma>) u)"])
-      apply (auto simp: G.Vrs_Sb G.Vrs_Map image_iff Eperm_Ector
+      apply (auto simp: G.Vrs_Sb G.Vrs_Map image_iff Eperm_Ector GMAP_def Gren_def
           dest: eta_inversion[rotated 2] eta'_inversion[rotated 2])
       done
     subgoal for e' u _
@@ -583,7 +642,7 @@ binder_inductive (no_auto_equiv) Efreee
       apply (rule exI[of _ "Gsub \<sigma> \<sigma> (Gmap (Eperm \<sigma>) (Eperm \<sigma>) u)"])
       apply (rule exI[of _ "\<sigma> a"])
       apply (auto simp: G.Vrs_Sb G.Vrs_Map G.Supp_Sb G.Supp_Map image_iff Eperm_Ector
-          Eperm_comp[THEN fun_cong, simplified] Eperm_id bij_implies_inject
+          Eperm_comp[THEN fun_cong, simplified] Eperm_id bij_implies_inject GMAP_def Gren_def
           dest: eta_inversion[rotated 2] eta'_inversion[rotated 2])
       done
     subgoal for e' u _
@@ -591,7 +650,7 @@ binder_inductive (no_auto_equiv) Efreee
       apply (rule exI[of _ "Gsub \<sigma> \<sigma> (Gmap (Eperm \<sigma>) (Eperm \<sigma>) u)"])
       apply (rule exI[of _ "\<sigma> a"])
       apply (auto simp: G.Vrs_Sb G.Vrs_Map G.Supp_Sb G.Supp_Map image_iff Eperm_Ector
-          Eperm_comp[THEN fun_cong, simplified] Eperm_id bij_implies_inject
+          Eperm_comp[THEN fun_cong, simplified] Eperm_id bij_implies_inject GMAP_def Gren_def
           dest: eta_inversion[rotated 2] eta'_inversion[rotated 2])
       done
     done
@@ -610,7 +669,7 @@ binder_inductive (no_auto_equiv) Efreee
       subgoal for _ u
         apply (rule exI[of _ a])
         apply (rule exI[of _ "Gsub id \<sigma> (Gmap (Eperm \<sigma>) id u)"])
-        apply (auto simp: G.Vrs_Sb G.Vrs_Map Ector_inject EVrs_Ector
+        apply (auto simp: G.Vrs_Sb G.Vrs_Map Ector_inject EVrs_Ector Gren_def
             intro!: exI[of _ \<sigma>] elim!: id_on_antimono
             dest: eta_inversion[rotated 2] eta'_inversion[rotated 2])
         done
@@ -618,7 +677,7 @@ binder_inductive (no_auto_equiv) Efreee
         apply (rule exI[of _ "Eperm \<sigma> e"])
         apply (rule exI[of _ "Gsub id \<sigma> (Gmap (Eperm \<sigma>) id u)"])
         apply (rule exI[of _ a])
-        apply (auto simp: G.Vrs_Sb G.Vrs_Map G.Supp_Sb G.Supp_Map Ector_inject EVrs_Ector id_onD[of _ \<sigma> a]
+        apply (auto simp: G.Vrs_Sb G.Vrs_Map G.Supp_Sb G.Supp_Map Ector_inject EVrs_Ector id_onD[of _ \<sigma> a] Gren_def
             intro!: exI[of _ \<sigma>] elim!: id_on_antimono
             dest: eta_inversion[rotated 2] eta'_inversion[rotated 2] prems(2)[of \<sigma> a e, rotated 2])
         done
@@ -626,7 +685,7 @@ binder_inductive (no_auto_equiv) Efreee
         apply (rule exI[of _ "e"])
         apply (rule exI[of _ "Gsub id \<sigma> (Gmap (Eperm \<sigma>) id u)"])
         apply (rule exI[of _ a])
-        apply (auto simp: G.Vrs_Sb G.Vrs_Map G.Supp_Sb G.Supp_Map Ector_inject EVrs_Ector
+        apply (auto simp: G.Vrs_Sb G.Vrs_Map G.Supp_Sb G.Supp_Map Ector_inject EVrs_Ector Gren_def
             intro!: exI[of _ \<sigma>] elim!: id_on_antimono
             dest: eta_inversion[rotated 2] eta'_inversion[rotated 2])
         done
@@ -647,14 +706,14 @@ binder_inductive (no_auto_equiv) Efree\<eta>
   subgoal for R B \<sigma> a e
     apply (elim disj_forward exE conjE; hypsubst_thin)
     subgoal for _
-      apply (auto simp: Eperm_Ector eta_natural)
+      apply (auto simp: Eperm_Ector eta_natural GMAP_def Gren_def)
       done
     subgoal for e' u _
       apply (rule exI[of _ "Eperm \<sigma> e'"])
       apply (rule exI[of _ "Gsub \<sigma> \<sigma> (Gmap (Eperm \<sigma>) (Eperm \<sigma>) u)"])
       apply (rule exI[of _ "\<sigma> a"])
       apply (auto simp: G.Vrs_Sb G.Vrs_Map G.Supp_Sb G.Supp_Map image_iff Eperm_Ector
-          Eperm_comp[THEN fun_cong, simplified] Eperm_id bij_implies_inject
+          Eperm_comp[THEN fun_cong, simplified] Eperm_id bij_implies_inject GMAP_def Gren_def
           dest: eta_inversion[rotated 2] eta'_inversion[rotated 2])
       done
     subgoal for e' u _
@@ -662,7 +721,7 @@ binder_inductive (no_auto_equiv) Efree\<eta>
       apply (rule exI[of _ "Gsub \<sigma> \<sigma> (Gmap (Eperm \<sigma>) (Eperm \<sigma>) u)"])
       apply (rule exI[of _ "\<sigma> a"])
       apply (auto simp: G.Vrs_Sb G.Vrs_Map G.Supp_Sb G.Supp_Map image_iff Eperm_Ector
-          Eperm_comp[THEN fun_cong, simplified] Eperm_id bij_implies_inject
+          Eperm_comp[THEN fun_cong, simplified] Eperm_id bij_implies_inject GMAP_def Gren_def
           dest: eta_inversion[rotated 2] eta'_inversion[rotated 2])
       done
     done
@@ -685,7 +744,7 @@ binder_inductive (no_auto_equiv) Efree\<eta>
         apply (rule exI[of _ "Eperm \<sigma> e"])
         apply (rule exI[of _ "Gsub id \<sigma> (Gmap (Eperm \<sigma>) id u)"])
         apply (rule exI[of _ a])
-        apply (auto simp: G.Vrs_Sb G.Vrs_Map G.Supp_Sb G.Supp_Map Ector_inject EVrs_Ector id_onD[of _ \<sigma> a]
+        apply (auto simp: G.Vrs_Sb G.Vrs_Map G.Supp_Sb G.Supp_Map Ector_inject EVrs_Ector id_onD[of _ \<sigma> a] Gren_def
             intro!: exI[of _ \<sigma>] elim!: id_on_antimono
             dest: eta_inversion[rotated 2] eta'_inversion[rotated 2] prems(2)[of \<sigma> a e, rotated 2])
         done
@@ -693,7 +752,7 @@ binder_inductive (no_auto_equiv) Efree\<eta>
         apply (rule exI[of _ "e"])
         apply (rule exI[of _ "Gsub id \<sigma> (Gmap (Eperm \<sigma>) id u)"])
         apply (rule exI[of _ a])
-        apply (auto simp: G.Vrs_Sb G.Vrs_Map G.Supp_Sb G.Supp_Map Ector_inject EVrs_Ector
+        apply (auto simp: G.Vrs_Sb G.Vrs_Map G.Supp_Sb G.Supp_Map Ector_inject EVrs_Ector Gren_def
             intro!: exI[of _ \<sigma>] elim!: id_on_antimono
             dest: eta_inversion[rotated 2] eta'_inversion[rotated 2])
         done
@@ -714,14 +773,14 @@ binder_inductive (no_auto_equiv) Efree\<eta>'
   subgoal for R B \<sigma> a e
     apply (elim disj_forward exE conjE; hypsubst_thin)
     subgoal for _
-      apply (auto simp: Eperm_Ector eta'_natural)
+      apply (auto simp: Eperm_Ector eta'_natural GMAP_def Gren_def)
       done
     subgoal for e' u _
       apply (rule exI[of _ "Eperm \<sigma> e'"])
       apply (rule exI[of _ "Gsub \<sigma> \<sigma> (Gmap (Eperm \<sigma>) (Eperm \<sigma>) u)"])
       apply (rule exI[of _ "\<sigma> a"])
       apply (auto simp: G.Vrs_Sb G.Vrs_Map G.Supp_Sb G.Supp_Map image_iff Eperm_Ector
-          Eperm_comp[THEN fun_cong, simplified] Eperm_id bij_implies_inject
+          Eperm_comp[THEN fun_cong, simplified] Eperm_id bij_implies_inject GMAP_def Gren_def
           dest: eta_inversion[rotated 2] eta'_inversion[rotated 2])
       done
     subgoal for e' u _
@@ -729,7 +788,7 @@ binder_inductive (no_auto_equiv) Efree\<eta>'
       apply (rule exI[of _ "Gsub \<sigma> \<sigma> (Gmap (Eperm \<sigma>) (Eperm \<sigma>) u)"])
       apply (rule exI[of _ "\<sigma> a"])
       apply (auto simp: G.Vrs_Sb G.Vrs_Map G.Supp_Sb G.Supp_Map image_iff Eperm_Ector
-          Eperm_comp[THEN fun_cong, simplified] Eperm_id bij_implies_inject
+          Eperm_comp[THEN fun_cong, simplified] Eperm_id bij_implies_inject GMAP_def Gren_def
           dest: eta_inversion[rotated 2] eta'_inversion[rotated 2])
       done
     done
@@ -752,7 +811,7 @@ binder_inductive (no_auto_equiv) Efree\<eta>'
         apply (rule exI[of _ "Eperm \<sigma> e"])
         apply (rule exI[of _ "Gsub id \<sigma> (Gmap (Eperm \<sigma>) id u)"])
         apply (rule exI[of _ a])
-        apply (auto simp: G.Vrs_Sb G.Vrs_Map G.Supp_Sb G.Supp_Map Ector_inject EVrs_Ector id_onD[of _ \<sigma> a]
+        apply (auto simp: G.Vrs_Sb G.Vrs_Map G.Supp_Sb G.Supp_Map Ector_inject EVrs_Ector id_onD[of _ \<sigma> a] Gren_def
             intro!: exI[of _ \<sigma>] elim!: id_on_antimono
             dest: eta_inversion[rotated 2] eta'_inversion[rotated 2] prems(2)[of \<sigma> a e, rotated 2])
         done
@@ -760,7 +819,7 @@ binder_inductive (no_auto_equiv) Efree\<eta>'
         apply (rule exI[of _ "e"])
         apply (rule exI[of _ "Gsub id \<sigma> (Gmap (Eperm \<sigma>) id u)"])
         apply (rule exI[of _ a])
-        apply (auto simp: G.Vrs_Sb G.Vrs_Map G.Supp_Sb G.Supp_Map Ector_inject EVrs_Ector
+        apply (auto simp: G.Vrs_Sb G.Vrs_Map G.Supp_Sb G.Supp_Map Ector_inject EVrs_Ector Gren_def
             intro!: exI[of _ \<sigma>] elim!: id_on_antimono
             dest: eta_inversion[rotated 2] eta'_inversion[rotated 2])
         done
@@ -775,9 +834,9 @@ definition "EFVrs\<eta>' e = {a. Efree\<eta>' a e}"
 lemma Esub_unique_fresh:
   assumes
     "|A| <o |UNIV::'a set|"
-    "|supp (\<delta> :: 'a \<Rightarrow> 'a :: var)| <o |UNIV::'a set|"
-    "|SSupp (Ector o \<eta>) (\<rho>::'a::var \<Rightarrow> 'a E)| <o |UNIV::'a set|"
-    "|SSupp (Ector o \<eta>') (\<rho>'::'a::var \<Rightarrow> 'a E)| <o |UNIV::'a set|"
+    "|supp (\<delta> :: 'a \<Rightarrow> 'a :: var_E_pre)| <o |UNIV::'a set|"
+    "|SSupp (Ector o \<eta>) (\<rho>::'a::var_E_pre \<Rightarrow> 'a E)| <o |UNIV::'a set|"
+    "|SSupp (Ector o \<eta>') (\<rho>'::'a::var_E_pre \<Rightarrow> 'a E)| <o |UNIV::'a set|"
     "\<And>a. h (Ector (\<eta> a)) = \<rho> a"
     "\<And>a. h (Ector (\<eta>' a)) = \<rho>' a"
     "\<And>u.
@@ -807,15 +866,15 @@ lemma Esub_unique_fresh:
         apply (cases "\<exists>a. u = \<eta>' a")
          apply (auto simp: Esub_Ector\<eta>' assms) []
         apply (rule disjI2)
-        apply (rule exI[where x="Gren \<delta> id u"])
-        apply (auto simp: assms Esub_Ector G.Map_Sb[THEN fun_cong, simplified] G.Sb_Inj)
+        apply (rule exI[where x="Gsub \<delta> id u"])
+        apply (auto simp: assms GMAP_def Gren_def G.Sb_Inj Esub_Ector G.Map_Sb[THEN fun_cong, simplified])
         done
       done
     done
   done
 
 lemma SSupp_comp_Esub_le:
-  assumes "|supp (\<delta> :: 'a \<Rightarrow> 'a::var)| <o |UNIV :: 'a set|"
+  assumes "|supp (\<delta> :: 'a \<Rightarrow> 'a::var_E_pre)| <o |UNIV :: 'a set|"
     "|SSupp (Ector \<circ> \<eta>) \<rho>| <o |UNIV :: 'a set|"
     "|SSupp (Ector \<circ> \<eta>') \<rho>'| <o |UNIV :: 'a set|"
   shows "SSupp (Ector \<circ> \<eta>) (Esub \<delta> \<rho> \<rho>' \<circ> \<rho>'') \<subseteq>
@@ -826,7 +885,7 @@ lemma SSupp_comp_Esub_le:
   by (auto simp: SSupp_def Esub_Ector\<eta> Esub_Ector\<eta>')
 
 lemma SSupp_comp_bound[simp]:
-  "|supp (\<delta> :: 'a \<Rightarrow> 'a::var)| <o |UNIV :: 'a set| \<Longrightarrow>
+  "|supp (\<delta> :: 'a \<Rightarrow> 'a::var_E_pre)| <o |UNIV :: 'a set| \<Longrightarrow>
   |SSupp (Ector \<circ> \<eta>) \<rho>| <o |UNIV :: 'a set| \<Longrightarrow>
   |SSupp (Ector \<circ> \<eta>') \<rho>'| <o |UNIV :: 'a set| \<Longrightarrow>
   |SSupp (Ector \<circ> \<eta>) \<rho>''| <o |UNIV :: 'a set| \<Longrightarrow>
@@ -837,7 +896,7 @@ lemma SSupp_comp_bound[simp]:
   done
 
 lemma SSupp_comp_bound'[simp]:
-  "|supp (\<delta> :: 'a \<Rightarrow> 'a::var)| <o |UNIV :: 'a set| \<Longrightarrow>
+  "|supp (\<delta> :: 'a \<Rightarrow> 'a::var_E_pre)| <o |UNIV :: 'a set| \<Longrightarrow>
   |SSupp (Ector \<circ> \<eta>) \<rho>| <o |UNIV :: 'a set| \<Longrightarrow>
   |SSupp (Ector \<circ> \<eta>') \<rho>'| <o |UNIV :: 'a set| \<Longrightarrow>
   |SSupp (Ector \<circ> \<eta>') \<rho>''| <o |UNIV :: 'a set| \<Longrightarrow>
@@ -879,30 +938,32 @@ lemma Efree\<eta>'_Efree: "Efree\<eta>' a e \<Longrightarrow> a \<in> EVrs e"
   by (induct e pred: Efree\<eta>') (auto simp: EVrs_Ector)
 
 lemma EFVrs_bd:
-  "|EFVrs (x :: 'a :: var E)| <o natLeq"
-  "|EFVrs\<eta> (x :: 'a :: var E)| <o natLeq"
-  "|EFVrs\<eta>' (x :: 'a :: var E)| <o natLeq"
+  "|EFVrs (x :: 'a :: var_E_pre E)| <o Gbd"
+  "|EFVrs\<eta> (x :: 'a :: var_E_pre E)| <o Gbd"
+  "|EFVrs\<eta>' (x :: 'a :: var_E_pre E)| <o Gbd"
     apply (meson EVrs_bd Efree_alt(1) Efreee_Efree card_of_subset_bound subset_eq)
    apply (meson EVrs_bd Efree_alt(2) Efree\<eta>_Efree card_of_subset_bound subset_eq)
   apply (meson EVrs_bd Efree_alt(3) Efree\<eta>'_Efree card_of_subset_bound subset_eq)
   done
 
 lemma EFVrs_bound[simp]:
-  "|EFVrs (x :: 'a :: var E)| <o |UNIV :: 'a set|"
-  "|EFVrs\<eta> (x :: 'a :: var E)| <o |UNIV :: 'a set|"
-  "|EFVrs\<eta>' (x :: 'a :: var E)| <o |UNIV :: 'a set|"
-  by (meson EFVrs_bd FType_pre.var_large ordLess_ordLeq_trans)+
+  "|EFVrs (x :: 'a :: var_E_pre E)| <o |UNIV :: 'a set|"
+  "|EFVrs\<eta> (x :: 'a :: var_E_pre E)| <o |UNIV :: 'a set|"
+  "|EFVrs\<eta>' (x :: 'a :: var_E_pre E)| <o |UNIV :: 'a set|"
+  using EFVrs_bd large' ordLess_ordLeq_trans by blast+
 
-lemma EFVrs_EsubI1:
+lemma EFVrs_EsubI1[OF _ _ _ _ refl]:
   assumes
     "z \<in> EFVrs e"
-    "|supp (\<delta> :: 'a \<Rightarrow> 'a::var)| <o |UNIV :: 'a set|"
+    "|supp (\<delta> :: 'a \<Rightarrow> 'a::var_E_pre)| <o |UNIV :: 'a set|"
     "|SSupp (Ector \<circ> \<eta>) \<rho>| <o |UNIV :: 'a set|"
     "|SSupp (Ector \<circ> \<eta>') \<rho>'| <o |UNIV :: 'a set|"
+     "e' = e"
   shows "\<delta> z \<in> EFVrs (Esub \<delta> \<rho> \<rho>' e)"
-  using assms(1) unfolding EFVrs_def mem_Collect_eq
-  apply (binder_induction z e avoiding: "imsupp \<delta>" "IImsupp' (Ector o \<eta>) EVrs \<rho>" "IImsupp' (Ector o \<eta>') EVrs \<rho>'" e rule: Efreee.strong_induct)
-       apply (auto simp: assms imsupp_supp_bound) [3]
+  using assms(1,5) unfolding EFVrs_def mem_Collect_eq
+  apply (binder_induction z e arbitrary: e' avoiding: "imsupp \<delta>" "IImsupp' (Ector o \<eta>) EVrs \<rho>" "IImsupp' (Ector o \<eta>') EVrs \<rho>'" "EVrs e'" rule: Efreee.strong_induct)
+        apply (auto simp: assms imsupp_supp_bound) [4]
+  apply hypsubst_thin
   subgoal for a u
     apply (subst Esub_Ector; (simp add: Int_Un_distrib assms(2-4))?)
     apply (rule Efreee.intros)
@@ -932,16 +993,17 @@ lemma EFVrs_EsubI1:
     done
   done
 
-lemma EFVrs_EsubI2:
+lemma EFVrs_EsubI2[OF _ _ _ _ _ refl]:
   assumes
     "a \<in> EFVrs\<eta> e" "z \<in> EFVrs (\<rho> a)"
-    "|supp (\<delta> :: 'a \<Rightarrow> 'a::var)| <o |UNIV :: 'a set|"
+    "|supp (\<delta> :: 'a \<Rightarrow> 'a::var_E_pre)| <o |UNIV :: 'a set|"
     "|SSupp (Ector \<circ> \<eta>) \<rho>| <o |UNIV :: 'a set|"
     "|SSupp (Ector \<circ> \<eta>') \<rho>'| <o |UNIV :: 'a set|"
+    "e' = e"
   shows "z \<in> EFVrs (Esub \<delta> \<rho> \<rho>' e)"
-  using assms(1,2) unfolding EFVrs_def EFVrs\<eta>_def mem_Collect_eq
-  apply (binder_induction a e avoiding: "imsupp \<delta>" "IImsupp' (Ector o \<eta>) EVrs \<rho>" "IImsupp' (Ector o \<eta>') EVrs \<rho>'" e rule: Efree\<eta>.strong_induct)
-       apply (auto simp: assms imsupp_supp_bound) [3]
+  using assms(1,2,6) unfolding EFVrs_def EFVrs\<eta>_def mem_Collect_eq
+  apply (binder_induction a e arbitrary: e' avoiding: "imsupp \<delta>" "IImsupp' (Ector o \<eta>) EVrs \<rho>" "IImsupp' (Ector o \<eta>') EVrs \<rho>'" "EVrs e'" rule: Efree\<eta>.strong_induct)
+        apply (auto simp: assms imsupp_supp_bound) [4]
   subgoal for a
     apply (subst Esub_Ector\<eta>; (simp add: Int_Un_distrib assms(3-5))?)
     done
@@ -953,7 +1015,7 @@ lemma EFVrs_EsubI2:
     apply (cases "\<rho> a = Ector (\<eta> a)")
      apply (metis Ector_eta_inj Efreee.cases GSupp_eta(1,2) empty_iff)
     apply (subgoal_tac "z \<in> IImsupp (Ector \<circ> \<eta>) EVrs \<rho>")
-     apply blast
+     apply fast
     apply (auto simp: IImsupp_def SSupp_def EFVrs\<eta>_def Efreee_Efree intro!: exI[of _ a]) []
     done
   subgoal for e' u a
@@ -964,16 +1026,17 @@ lemma EFVrs_EsubI2:
     done
   done
 
-lemma EFVrs_EsubI3:
+lemma EFVrs_EsubI3[OF _ _ _ _ _ refl]:
   assumes
     "a \<in> EFVrs\<eta>' e" "z \<in> EFVrs (\<rho>' a)"
-    "|supp (\<delta> :: 'a \<Rightarrow> 'a::var)| <o |UNIV :: 'a set|"
+    "|supp (\<delta> :: 'a \<Rightarrow> 'a::var_E_pre)| <o |UNIV :: 'a set|"
     "|SSupp (Ector \<circ> \<eta>) \<rho>| <o |UNIV :: 'a set|"
     "|SSupp (Ector \<circ> \<eta>') \<rho>'| <o |UNIV :: 'a set|"
+    "e' = e"
   shows "z \<in> EFVrs (Esub \<delta> \<rho> \<rho>' e)"
-  using assms(1,2) unfolding EFVrs_def EFVrs\<eta>'_def mem_Collect_eq
-  apply (binder_induction a e avoiding: "imsupp \<delta>" "IImsupp' (Ector o \<eta>) EVrs \<rho>" "IImsupp' (Ector o \<eta>') EVrs \<rho>'" e rule: Efree\<eta>'.strong_induct)
-       apply (auto simp: assms imsupp_supp_bound) [3]
+  using assms(1,2,6) unfolding EFVrs_def EFVrs\<eta>'_def mem_Collect_eq
+  apply (binder_induction a e arbitrary: e' avoiding: "imsupp \<delta>" "IImsupp' (Ector o \<eta>) EVrs \<rho>" "IImsupp' (Ector o \<eta>') EVrs \<rho>'" "EVrs e'" rule: Efree\<eta>'.strong_induct)
+       apply (auto simp: assms imsupp_supp_bound) [4]
   subgoal for a
     apply (subst Esub_Ector\<eta>'; (simp add: Int_Un_distrib assms(3-5))?)
     done
@@ -985,7 +1048,7 @@ lemma EFVrs_EsubI3:
     apply (cases "\<rho>' a = Ector (\<eta>' a)")
      apply (metis Ector_eta'_inj Efreee.cases GSupp_eta'(1,2) empty_iff)
     apply (subgoal_tac "z \<in> IImsupp (Ector \<circ> \<eta>') EVrs \<rho>'")
-     apply blast
+     apply fast
     apply (auto simp: IImsupp_def SSupp_def EFVrs\<eta>'_def Efreee_Efree intro!: exI[of _ a]) []
     done
   subgoal for e' u a
@@ -999,7 +1062,7 @@ lemma EFVrs_EsubI3:
 lemma EFVrs_EsubD:
   assumes
     "z \<in> EFVrs (Esub \<delta> \<rho> \<rho>' e)"
-    "|supp (\<delta> :: 'a \<Rightarrow> 'a::var)| <o |UNIV :: 'a set|"
+    "|supp (\<delta> :: 'a \<Rightarrow> 'a::var_E_pre)| <o |UNIV :: 'a set|"
     "|SSupp (Ector \<circ> \<eta>) \<rho>| <o |UNIV :: 'a set|"
     "|SSupp (Ector \<circ> \<eta>') \<rho>'| <o |UNIV :: 'a set|"
   shows "
@@ -1108,16 +1171,17 @@ lemma EFVrs_EsubD:
     done
   done
 
-lemma EFVrs\<eta>_EsubI2:
+lemma EFVrs\<eta>_EsubI2[OF _ _ _ _ _ refl]:
   assumes
     "a \<in> EFVrs\<eta> e" "z \<in> EFVrs\<eta> (\<rho> a)"
-    "|supp (\<delta> :: 'a \<Rightarrow> 'a::var)| <o |UNIV :: 'a set|"
+    "|supp (\<delta> :: 'a \<Rightarrow> 'a::var_E_pre)| <o |UNIV :: 'a set|"
     "|SSupp (Ector \<circ> \<eta>) \<rho>| <o |UNIV :: 'a set|"
     "|SSupp (Ector \<circ> \<eta>') \<rho>'| <o |UNIV :: 'a set|"
+    "e' = e"
   shows "z \<in> EFVrs\<eta> (Esub \<delta> \<rho> \<rho>' e)"
-  using assms(1,2) unfolding EFVrs\<eta>_def mem_Collect_eq
-  apply (binder_induction a e avoiding: "imsupp \<delta>" "IImsupp' (Ector o \<eta>) EVrs \<rho>" "IImsupp' (Ector o \<eta>') EVrs \<rho>'" e rule: Efree\<eta>.strong_induct)
-       apply (auto simp: assms imsupp_supp_bound) [3]
+  using assms(1,2,6) unfolding EFVrs\<eta>_def mem_Collect_eq
+  apply (binder_induction a e arbitrary: e' avoiding: "imsupp \<delta>" "IImsupp' (Ector o \<eta>) EVrs \<rho>" "IImsupp' (Ector o \<eta>') EVrs \<rho>'" "EVrs e'" rule: Efree\<eta>.strong_induct)
+        apply (auto simp: assms imsupp_supp_bound) [4]
   subgoal for a
     apply (subst Esub_Ector\<eta>; (simp add: Int_Un_distrib assms(3-5))?)
     done
@@ -1129,7 +1193,7 @@ lemma EFVrs\<eta>_EsubI2:
     apply (cases "\<rho> a = Ector (\<eta> a)")
      apply (simp add: EFVrs\<eta>_Ector_eta Efree_alt(2))
     apply (subgoal_tac "z \<in> IImsupp (Ector \<circ> \<eta>) EVrs \<rho>")
-     apply blast
+     apply fast
     apply (auto simp: IImsupp_def SSupp_def EFVrs\<eta>_def Efree\<eta>_Efree intro!: exI[of _ a]) []
     done
   subgoal for e' u a
@@ -1140,16 +1204,17 @@ lemma EFVrs\<eta>_EsubI2:
     done
   done
 
-lemma EFVrs\<eta>_EsubI3:
+lemma EFVrs\<eta>_EsubI3[OF _ _ _ _ _ refl]:
   assumes
     "a \<in> EFVrs\<eta>' e" "z \<in> EFVrs\<eta> (\<rho>' a)"
-    "|supp (\<delta> :: 'a \<Rightarrow> 'a::var)| <o |UNIV :: 'a set|"
+    "|supp (\<delta> :: 'a \<Rightarrow> 'a::var_E_pre)| <o |UNIV :: 'a set|"
     "|SSupp (Ector \<circ> \<eta>) \<rho>| <o |UNIV :: 'a set|"
     "|SSupp (Ector \<circ> \<eta>') \<rho>'| <o |UNIV :: 'a set|"
+    "e' = e"
   shows "z \<in> EFVrs\<eta> (Esub \<delta> \<rho> \<rho>' e)"
-  using assms(1,2) unfolding EFVrs\<eta>_def EFVrs\<eta>'_def mem_Collect_eq
-  apply (binder_induction a e avoiding: "imsupp \<delta>" "IImsupp' (Ector o \<eta>) EVrs \<rho>" "IImsupp' (Ector o \<eta>') EVrs \<rho>'" e rule: Efree\<eta>'.strong_induct)
-       apply (auto simp: assms imsupp_supp_bound) [3]
+  using assms(1,2,6) unfolding EFVrs\<eta>_def EFVrs\<eta>'_def mem_Collect_eq
+  apply (binder_induction a e arbitrary: e' avoiding: "imsupp \<delta>" "IImsupp' (Ector o \<eta>) EVrs \<rho>" "IImsupp' (Ector o \<eta>') EVrs \<rho>'" "EVrs e'" rule: Efree\<eta>'.strong_induct)
+       apply (auto simp: assms imsupp_supp_bound) [4]
   subgoal for a
     apply (subst Esub_Ector\<eta>'; (simp add: Int_Un_distrib assms(3-5))?)
     done
@@ -1161,7 +1226,7 @@ lemma EFVrs\<eta>_EsubI3:
     apply (cases "\<rho>' a = Ector (\<eta>' a)")
      apply (metis Ector_eta'_inj Efree\<eta>.cases GSupp_eta'(1,2) empty_iff eta_distinct)
     apply (subgoal_tac "z \<in> IImsupp (Ector \<circ> \<eta>') EVrs \<rho>'")
-     apply blast
+     apply fast
     apply (auto simp: IImsupp_def SSupp_def EFVrs\<eta>'_def Efree\<eta>_Efree intro!: exI[of _ a]) []
     done
   subgoal for e' u a
@@ -1175,7 +1240,7 @@ lemma EFVrs\<eta>_EsubI3:
 lemma EFVrs\<eta>_EsubD:
   assumes
     "z \<in> EFVrs\<eta> (Esub \<delta> \<rho> \<rho>' e)"
-    "|supp (\<delta> :: 'a \<Rightarrow> 'a::var)| <o |UNIV :: 'a set|"
+    "|supp (\<delta> :: 'a \<Rightarrow> 'a::var_E_pre)| <o |UNIV :: 'a set|"
     "|SSupp (Ector \<circ> \<eta>) \<rho>| <o |UNIV :: 'a set|"
     "|SSupp (Ector \<circ> \<eta>') \<rho>'| <o |UNIV :: 'a set|"
   shows "
@@ -1263,16 +1328,17 @@ lemma EFVrs\<eta>_EsubD:
     done
   done
 
-lemma EFVrs\<eta>'_EsubI2:
+lemma EFVrs\<eta>'_EsubI2[OF _ _ _ _ _ refl]:
   assumes
     "a \<in> EFVrs\<eta> e" "z \<in> EFVrs\<eta>' (\<rho> a)"
-    "|supp (\<delta> :: 'a \<Rightarrow> 'a::var)| <o |UNIV :: 'a set|"
+    "|supp (\<delta> :: 'a \<Rightarrow> 'a::var_E_pre)| <o |UNIV :: 'a set|"
     "|SSupp (Ector \<circ> \<eta>) \<rho>| <o |UNIV :: 'a set|"
     "|SSupp (Ector \<circ> \<eta>') \<rho>'| <o |UNIV :: 'a set|"
+    "e' = e"
   shows "z \<in> EFVrs\<eta>' (Esub \<delta> \<rho> \<rho>' e)"
-  using assms(1,2) unfolding EFVrs\<eta>_def EFVrs\<eta>'_def mem_Collect_eq
-  apply (binder_induction a e avoiding: "imsupp \<delta>" "IImsupp' (Ector o \<eta>) EVrs \<rho>" "IImsupp' (Ector o \<eta>') EVrs \<rho>'" e rule: Efree\<eta>.strong_induct)
-       apply (auto simp: assms imsupp_supp_bound) [3]
+  using assms(1,2,6) unfolding EFVrs\<eta>_def EFVrs\<eta>'_def mem_Collect_eq
+  apply (binder_induction a e arbitrary: e' avoiding: "imsupp \<delta>" "IImsupp' (Ector o \<eta>) EVrs \<rho>" "IImsupp' (Ector o \<eta>') EVrs \<rho>'" "EVrs e'" rule: Efree\<eta>.strong_induct)
+       apply (auto simp: assms imsupp_supp_bound) [4]
   subgoal for a
     apply (subst Esub_Ector\<eta>; (simp add: Int_Un_distrib assms(3-5))?)
     done
@@ -1284,7 +1350,7 @@ lemma EFVrs\<eta>'_EsubI2:
     apply (cases "\<rho> a = Ector (\<eta> a)")
      apply (metis Ector_eta_inj Efree\<eta>'.cases GSupp_eta(1,2) empty_iff eta_distinct)
     apply (subgoal_tac "z \<in> IImsupp (Ector \<circ> \<eta>) EVrs \<rho>")
-     apply blast
+     apply fast
     apply (auto simp: IImsupp_def SSupp_def EFVrs\<eta>'_def Efree\<eta>'_Efree intro!: exI[of _ a]) []
     done
   subgoal for e' u a
@@ -1295,16 +1361,17 @@ lemma EFVrs\<eta>'_EsubI2:
     done
   done
 
-lemma EFVrs\<eta>'_EsubI3:
+lemma EFVrs\<eta>'_EsubI3[OF _ _ _ _ _ refl]:
   assumes
     "a \<in> EFVrs\<eta>' e" "z \<in> EFVrs\<eta>' (\<rho>' a)"
-    "|supp (\<delta> :: 'a \<Rightarrow> 'a::var)| <o |UNIV :: 'a set|"
+    "|supp (\<delta> :: 'a \<Rightarrow> 'a::var_E_pre)| <o |UNIV :: 'a set|"
     "|SSupp (Ector \<circ> \<eta>) \<rho>| <o |UNIV :: 'a set|"
     "|SSupp (Ector \<circ> \<eta>') \<rho>'| <o |UNIV :: 'a set|"
+    "e' = e"
   shows "z \<in> EFVrs\<eta>' (Esub \<delta> \<rho> \<rho>' e)"
-  using assms(1,2) unfolding EFVrs\<eta>'_def mem_Collect_eq
-  apply (binder_induction a e avoiding: "imsupp \<delta>" "IImsupp' (Ector o \<eta>) EVrs \<rho>" "IImsupp' (Ector o \<eta>') EVrs \<rho>'" e rule: Efree\<eta>'.strong_induct)
-       apply (auto simp: assms imsupp_supp_bound) [3]
+  using assms(1,2,6) unfolding EFVrs\<eta>'_def mem_Collect_eq
+  apply (binder_induction a e arbitrary: e' avoiding: "imsupp \<delta>" "IImsupp' (Ector o \<eta>) EVrs \<rho>" "IImsupp' (Ector o \<eta>') EVrs \<rho>'" "EVrs e'" rule: Efree\<eta>'.strong_induct)
+       apply (auto simp: assms imsupp_supp_bound) [4]
   subgoal for a
     apply (subst Esub_Ector\<eta>'; (simp add: Int_Un_distrib assms(3-5))?)
     done
@@ -1316,7 +1383,7 @@ lemma EFVrs\<eta>'_EsubI3:
     apply (cases "\<rho>' a = Ector (\<eta>' a)")
      apply (simp add: EFVrs\<eta>'_Ector_eta' Efree_alt(3))
     apply (subgoal_tac "z \<in> IImsupp (Ector \<circ> \<eta>') EVrs \<rho>'")
-     apply blast
+     apply fast
     apply (auto simp: IImsupp_def SSupp_def EFVrs\<eta>'_def Efree\<eta>'_Efree intro!: exI[of _ a]) []
     done
   subgoal for e' u a
@@ -1330,7 +1397,7 @@ lemma EFVrs\<eta>'_EsubI3:
 lemma EFVrs\<eta>'_EsubD:
   assumes
     "z \<in> EFVrs\<eta>' (Esub \<delta> \<rho> \<rho>' e)"
-    "|supp (\<delta> :: 'a \<Rightarrow> 'a::var)| <o |UNIV :: 'a set|"
+    "|supp (\<delta> :: 'a \<Rightarrow> 'a::var_E_pre)| <o |UNIV :: 'a set|"
     "|SSupp (Ector \<circ> \<eta>) \<rho>| <o |UNIV :: 'a set|"
     "|SSupp (Ector \<circ> \<eta>') \<rho>'| <o |UNIV :: 'a set|"
   shows "
@@ -1420,30 +1487,30 @@ lemma EFVrs\<eta>'_EsubD:
 
 (*
 declare [[goals_limit=18]]
-pbmv_monad "'a::var E"
+pbmv_monad "'a::var_E_pre E"
   Sbs: Esub
   RVrs: EFVrs
   Injs: "Ector o \<eta>" "Ector o \<eta>'"
   Vrs: EFVrs\<eta> EFVrs\<eta>'
-  bd: natLeq
+  bd: Gbd
   oops
 *)
 
 lemma E_pbmv_axioms:
- "infinite_regular_card_order natLeq"
+ "infinite_regular_card_order Gbd"
  "Esub id (Ector \<circ> \<eta>) (Ector \<circ> \<eta>') = id"
  "\<And>f \<rho>1 \<rho>2.
-       |supp (f :: 'a :: var \<Rightarrow> 'a)| <o |UNIV :: 'a set| \<Longrightarrow>
+       |supp (f :: 'a :: var_E_pre \<Rightarrow> 'a)| <o |UNIV :: 'a set| \<Longrightarrow>
        |SSupp (Ector \<circ> \<eta>) \<rho>1| <o |UNIV :: 'a set| \<Longrightarrow>
        |SSupp (Ector \<circ> \<eta>') \<rho>2| <o |UNIV :: 'a set| \<Longrightarrow>
        Esub f \<rho>1 \<rho>2 \<circ> (Ector \<circ> \<eta>) = \<rho>1"
  "\<And>f \<rho>1 \<rho>2.
-       |supp (f :: 'a :: var \<Rightarrow> 'a)| <o |UNIV :: 'a set| \<Longrightarrow>
+       |supp (f :: 'a :: var_E_pre \<Rightarrow> 'a)| <o |UNIV :: 'a set| \<Longrightarrow>
        |SSupp (Ector \<circ> \<eta>) \<rho>1| <o |UNIV :: 'a set| \<Longrightarrow>
        |SSupp (Ector \<circ> \<eta>') \<rho>2| <o |UNIV :: 'a set| \<Longrightarrow>
        Esub f \<rho>1 \<rho>2 \<circ> (Ector \<circ> \<eta>') = \<rho>2"
  "\<And>g \<rho>'1 \<rho>'2 f \<rho>1 \<rho>2.
-       |supp (f :: 'a :: var \<Rightarrow> 'a)| <o |UNIV :: 'a set| \<Longrightarrow>
+       |supp (f :: 'a :: var_E_pre \<Rightarrow> 'a)| <o |UNIV :: 'a set| \<Longrightarrow>
        |SSupp (Ector \<circ> \<eta>) \<rho>1| <o |UNIV :: 'a set| \<Longrightarrow>
        |SSupp (Ector \<circ> \<eta>') \<rho>2| <o |UNIV :: 'a set| \<Longrightarrow>
        |supp g| <o |UNIV :: 'a set| \<Longrightarrow>
@@ -1451,9 +1518,9 @@ lemma E_pbmv_axioms:
        |SSupp (Ector \<circ> \<eta>') \<rho>'2| <o |UNIV :: 'a set| \<Longrightarrow>
        Esub g \<rho>'1 \<rho>'2 \<circ> Esub f \<rho>1 \<rho>2 =
        Esub (g \<circ> f) (Esub g \<rho>'1 \<rho>'2 \<circ> \<rho>1) (Esub g \<rho>'1 \<rho>'2 \<circ> \<rho>2)"
- "\<And>x. |EFVrs x| <o natLeq"
- "\<And>x. |EFVrs\<eta> x| <o natLeq"
- "\<And>x. |EFVrs\<eta>' x| <o natLeq"
+ "\<And>x. |EFVrs x| <o Gbd"
+ "\<And>x. |EFVrs\<eta> x| <o Gbd"
+ "\<And>x. |EFVrs\<eta>' x| <o Gbd"
  "\<And>a. EFVrs ((Ector \<circ> \<eta>) a) = {}"
  "\<And>a. EFVrs ((Ector \<circ> \<eta>') a) = {}"
  "\<And>a. EFVrs\<eta> ((Ector \<circ> \<eta>) a) = {a}"
@@ -1461,26 +1528,26 @@ lemma E_pbmv_axioms:
  "\<And>a. EFVrs\<eta>' ((Ector \<circ> \<eta>) a) = {}"
  "\<And>a. EFVrs\<eta>' ((Ector \<circ> \<eta>') a) = {a}"
  "\<And>f \<rho>1 \<rho>2 x.
-        |supp (f :: 'a :: var \<Rightarrow> 'a)| <o |UNIV :: 'a set| \<Longrightarrow>
+        |supp (f :: 'a :: var_E_pre \<Rightarrow> 'a)| <o |UNIV :: 'a set| \<Longrightarrow>
         |SSupp (Ector \<circ> \<eta>) \<rho>1| <o |UNIV :: 'a set| \<Longrightarrow>
         |SSupp (Ector \<circ> \<eta>') \<rho>2| <o |UNIV :: 'a set| \<Longrightarrow>
         EFVrs (Esub f \<rho>1 \<rho>2 x) =
         f ` EFVrs x \<union>
         ((\<Union>x\<in>EFVrs\<eta> x. EFVrs (\<rho>1 x)) \<union> (\<Union>x\<in>EFVrs\<eta>' x. EFVrs (\<rho>2 x)))"
  "\<And>f \<rho>1 \<rho>2 x.
-        |supp (f :: 'a :: var \<Rightarrow> 'a)| <o |UNIV :: 'a set| \<Longrightarrow>
+        |supp (f :: 'a :: var_E_pre \<Rightarrow> 'a)| <o |UNIV :: 'a set| \<Longrightarrow>
         |SSupp (Ector \<circ> \<eta>) \<rho>1| <o |UNIV :: 'a set| \<Longrightarrow>
         |SSupp (Ector \<circ> \<eta>') \<rho>2| <o |UNIV :: 'a set| \<Longrightarrow>
         EFVrs\<eta> (Esub f \<rho>1 \<rho>2 x) =
         (\<Union>x\<in>EFVrs\<eta> x. EFVrs\<eta> (\<rho>1 x)) \<union> (\<Union>x\<in>EFVrs\<eta>' x. EFVrs\<eta> (\<rho>2 x))"
  "\<And>f \<rho>1 \<rho>2 x.
-        |supp (f :: 'a :: var \<Rightarrow> 'a)| <o |UNIV :: 'a set| \<Longrightarrow>
+        |supp (f :: 'a :: var_E_pre \<Rightarrow> 'a)| <o |UNIV :: 'a set| \<Longrightarrow>
         |SSupp (Ector \<circ> \<eta>) \<rho>1| <o |UNIV :: 'a set| \<Longrightarrow>
         |SSupp (Ector \<circ> \<eta>') \<rho>2| <o |UNIV :: 'a set| \<Longrightarrow>
         EFVrs\<eta>' (Esub f \<rho>1 \<rho>2 x) =
         (\<Union>x\<in>EFVrs\<eta> x. EFVrs\<eta>' (\<rho>1 x)) \<union> (\<Union>x\<in>EFVrs\<eta>' x. EFVrs\<eta>' (\<rho>2 x))"
  "\<And>f \<rho>1 \<rho>2 g \<rho>'1 \<rho>'2 x.
-        |supp (f :: 'a :: var \<Rightarrow> 'a)| <o |UNIV :: 'a set| \<Longrightarrow>
+        |supp (f :: 'a :: var_E_pre \<Rightarrow> 'a)| <o |UNIV :: 'a set| \<Longrightarrow>
         |SSupp (Ector \<circ> \<eta>) \<rho>1| <o |UNIV :: 'a set| \<Longrightarrow>
         |SSupp (Ector \<circ> \<eta>') \<rho>2| <o |UNIV :: 'a set| \<Longrightarrow>
         |supp g| <o |UNIV :: 'a set| \<Longrightarrow>
@@ -1491,7 +1558,7 @@ lemma E_pbmv_axioms:
         (\<And>a. a \<in> EFVrs\<eta>' x \<Longrightarrow> \<rho>2 a = \<rho>'2 a) \<Longrightarrow>
         Esub f \<rho>1 \<rho>2 x = Esub g \<rho>'1 \<rho>'2 x"
   subgoal
-    by (rule infinite_regular_card_order_natLeq)
+    by (rule G.infinite_regular_card_order)
   subgoal
     apply (rule Esub_unique_fresh[symmetric, where A="{}"])
           apply (simp_all add: G.Sb_Inj G.Map_id)
@@ -1507,7 +1574,7 @@ lemma E_pbmv_axioms:
           apply (simp_all add: supp_comp_bound Esub_Ector\<eta> Esub_Ector\<eta>' Esub_Ector Un_bound
         imsupp_supp_bound Int_Un_distrib)
     apply (subst Esub_Ector;
-        (simp add: G.Vrs_Sb G.Vrs_Map G.Supp_Sb G.Supp_Map Int_Un_distrib G.Map_comp[THEN fun_cong, simplified]
+        (simp add: EVrs_Ector G.Vrs_Sb G.Vrs_Map G.Supp_Sb G.Supp_Map Int_Un_distrib G.Map_comp[THEN fun_cong, simplified]
           G.Map_Sb[THEN fun_cong, simplified] G.Sb_comp[THEN fun_cong, simplified])?)
       apply (rule conjI)
     apply (metis Int_commute Int_image_imsupp)
@@ -1545,6 +1612,7 @@ lemma E_pbmv_axioms:
           and P = "\<lambda>e. (\<forall>a \<in> EFVrs e. \<delta>1 a = \<delta>2 a) \<and> (\<forall>a \<in> EFVrs\<eta> e. \<rho>1 a = \<rho>2 a) \<and> (\<forall>a \<in> EFVrs\<eta>' e. \<rho>1' a = \<rho>2' a)", rotated -1])
      apply blast
     subgoal premises prems for e
+      thm prems
       apply (insert prems(1-6,10-))
       apply (cases "\<exists>a. e = Ector (\<eta> a)")
        apply (auto simp: Esub_Ector\<eta> EFVrs\<eta>_Ector_eta) []
@@ -1560,9 +1628,9 @@ lemma E_pbmv_axioms:
       apply (erule exE conjE)+
       apply hypsubst_thin
       subgoal for u
-        apply (rule exI[where x="Gren \<delta>2 id u"])
+        apply (rule exI[where x="Gsub \<delta>2 id u"])
         apply (simp add: G.Supp_Sb Esub_Ector Ector_eta_inj Ector_eta'_inj
-            G.Map_Sb[THEN fun_cong, simplified] G.Sb_Inj)
+            G.Map_Sb[THEN fun_cong, simplified] GMAP_def Gren_def G.Sb_Inj)
         apply (intro conjI ballI)
               apply (rule arg_cong[where f = Ector])
               apply (rule G.Sb_cong; (simp add: G.Vrs_Map)?)
@@ -1586,5 +1654,6 @@ lemma E_pbmv_axioms:
       done
     done
   done
+unused_thms
 
 end
